nola/examples/type/rules/conv.v
@@ -43,8 +43,8 @@ Section conv.
   Lemma ttrans_mono_lev `{! i ≤ⁿ i'} {d j T k U} :
     T ==>{j,k}(i,d) U → T ==>{j,k}(i',d) U.
   Proof.
-    iIntros (TU ???) "T". iApply fupdw_expand; [|by iApply TU].
-    iApply tinv_wsat_incl.
+    iIntros (TU ???) "T". iApply fupdw_incl; [apply wsat_incl_tinv|].
+    by iApply TU.
   Qed.
 
   (** [⊑] into [==>] *)
@@ -100,9 +100,9 @@ Section conv.
   Proof.
     move=> T'T UU' ? /=. do 3 f_equiv. iIntros "hor T'".
     rewrite !twpw_tinv_wsat_lt_tinv_wsat. iMod (T'T with "T'") as "T"; [done|].
-    iDestruct ("hor" with "T") as "wp".
-    iDestruct (twpw_expand with "[] wp") as "?"; [iApply tinv_wsat_incl|].
-    iApply twpw_fupdw_nonval; [done|]. iStopProof. do 2 f_equiv. by iApply UU'.
+    iDestruct ("hor" with "T") as "wp". iApply twpw_fupdw_nonval; [done|].
+    iApply twpw_incl; [apply wsat_incl_tinv|]. iStopProof. do 2 f_equiv.
+    by iApply UU'.
   Qed.
   Lemma teqv_fun `{! j ≤ⁿ i, ! j ≤ⁿ i'} {d T U T' U'} :
     T <==>(j,d) T' →  U <==>(j,d) U' →  T →(j) U ≃{i,i'}(d) T' →(j) U'.
@@ -116,7 +116,7 @@ Section conv.
     ninv tguardN (tinvd_guard T v) -∗ tguard d (i:=i) T v.
   Proof.
     iIntros "#inv !>". iApply (derivy_intro (d:=d))=>/=. iIntros (?????).
-    iApply fupdw_expand; [iApply (tinv_wsat_tninv_wsat (M:=S i))|].
+    iApply fupdw_incl; [apply wsat_incl_tinv_tninv|].
     iMod (ninv_acc with "inv") as "/=[#$ cl]"; [done|]. by iApply "cl".
   Qed.
   Lemma ttrans_guard_intro `{!tderivy Σ ih d, ! i <ⁿ j} {k T} :
@@ -124,7 +124,7 @@ Section conv.
   Proof.
     iIntros (???) "/= #?". iApply fupdw_tinv_wsat_le. iIntros (?).
     have ?: i <ⁿ L by apply (nlt_nle_trans _ _).
-    iApply fupdw_expand; [iApply (tinv_wsat_tninv_wsat (M:=j))|].
+    iApply fupdw_incl; [apply wsat_incl_tinv_tninv|].
     iMod (ninv_alloc (P:=tinvd_guard T _) with "[]") as "inv"; [done|].
     iApply (ninv_tguard with "inv").
   Qed.
@@ -144,7 +144,7 @@ Section conv.
     move=> TU ? /=. unfold tguard. f_equiv. iIntros "T".
     iApply (derivy_map (d:=d) with "[] T"). iIntros (?? IH) "/= big % %inE".
     iApply fupdw_trans. assert (S j ≤ⁿ S j') by exact _.
-    iApply fupdw_expand; [iApply tinv_wsat_incl|]. iMod ("big" $! _ inE) as "T".
+    iApply fupdw_incl; [apply wsat_incl_tinv|]. iMod ("big" $! _ inE) as "T".
     iModIntro. by iMod (TU _ _ IH with "T") as "$"; [solve_ndisj|].
   Qed.
   Lemma teqv_guard `{!tderivy Σ ih d} {i i' j T U} :
@@ -165,12 +165,12 @@ Section conv.
     move=> TU ? /=. unfold tref. do 4 f_equiv. iIntros "T".
     iApply (derivy_map (d:=d) with "[] T"). iIntros (?? IH) "/= big".
     iApply fupdw_trans. assert (S j ≤ⁿ S j') by exact _.
-    iApply fupdw_expand; [iApply tinv_wsat_incl|].
+    iApply fupdw_incl; [apply wsat_incl_tinv|].
     iMod "big" as (?) "(↦ & T & cl)". iModIntro.
     iMod (proj1 (TU _ _ IH) with "T") as "U"; [solve_ndisj|]. iModIntro.
     iExists _. iFrame "↦ U". iIntros (?) "↦ U".
     iMod (proj2 (TU _ _ IH) with "U") as "T"; [solve_ndisj|].
-    iApply fupdw_expand; [iApply tinv_wsat_incl|]. by iMod ("cl" with "↦ T").
+    iApply fupdw_incl; [apply wsat_incl_tinv|]. by iMod ("cl" with "↦ T").
   Qed.
   Lemma teqv_ref `{!tderivy Σ ih d} {o i i' j T U} :
     (∀ `{!tderivy Σ ih d'}, ih d' → T <==>(S j,d') U) →
