nola/examples/type/rules/ref.v
@@ -11,11 +11,10 @@ Section eref.
     ninv trefN (tinvd_ref l T) ⊢ tref d (i:=i) l T.
   Proof.
     iIntros "#inv !>". iApply (derivy_intro (d:=d))=>/=. iIntros (???).
-    iApply fupdw_expand; [iApply (tinv_wsat_tninv_wsat (M:=S i))|].
     iMod (ninv_acc with "inv") as "/=[(%& ↦ & T) cl]"; [done|].
     iModIntro. iExists _. iFrame "↦ T". iIntros (?) "↦ T".
-    iApply fupdw_expand; [iApply (tinv_wsat_tninv_wsat (M:=S i))|]. iApply "cl".
-    iExists _. iFrame.
+    iApply fupdw_incl; [apply wsat_incl_tinv_tninv|]. iApply "cl". iExists _.
+    iFrame.
   Qed.
   Lemma texpr_ref_ref `{! i <ⁿ j} {e k T} :
     e :ᵉ(j) T ⊢ ref e :ᵉ{k}(j) ref{i,nil}: T.
@@ -23,7 +22,7 @@ Section eref.
     iIntros "?". unfold texpr. wp_bind e. iApply (twp_wand with "[$]").
     iIntros (?) ">#?". wp_alloc l as "↦". iModIntro. iApply fupdw_tinv_wsat_le.
     iIntros (?). have ?: i <ⁿ L by apply (nlt_nle_trans _ _).
-    iApply fupdw_expand; [iApply (tinv_wsat_tninv_wsat (M:=j))|].
+    iApply fupdw_incl; [apply (wsat_incl_tinv_tninv (M:=j))|].
     iMod (ninv_alloc (P:=tinvd_ref l T) with "[↦]") as "?";
       [iExists _; by iFrame|].
     iModIntro=>/=. iExists _. iSplit; [done|]. iApply ninv_tref.
@@ -52,11 +51,9 @@ Section eref.
     iIntros (?) "/= >(%&->& ref)". rewrite Loc.add_0.
     iApply (twpw_atomic (e:=! _)); [done|]. iApply fupdw_tinv_wsat_le.
     iIntros (?). have ? : i <ⁿ L by exact (nlt_nle_trans _ _).
-    have ? : S i ≤ⁿ j by done. iApply fupdw_expand; [iApply tinv_wsat_incl|].
-    iDestruct tderiv_sound as "→".
+    iDestruct tderiv_sound as "→". have ? : S i ≤ⁿ j by done.
     iMod ("→" with "ref") as (?) "(↦ & #T & cl)". iModIntro. wp_load.
-    iModIntro. iApply fupdw_expand; [iApply tinv_wsat_incl|].
-    by iMod ("cl" with "↦ T") as "_".
+    iModIntro. by iMod ("cl" with "↦ T") as "_".
   Qed.
 
   (** Store to [ref[ ]] *)
@@ -68,11 +65,9 @@ Section eref.
     iIntros (?) "/= >(%&->& ref)". rewrite Loc.add_0.
     iApply (twpw_atomic (e:=_ <- _)); [done|]. iApply fupdw_tinv_wsat_le.
     iIntros (?). have ? : i <ⁿ L by exact (nlt_nle_trans _ _).
-    have ? : S i ≤ⁿ j by done. iApply fupdw_expand; [iApply tinv_wsat_incl|].
-    iDestruct tderiv_sound as "→".
+    iDestruct tderiv_sound as "→". have ? : S i ≤ⁿ j by done.
     iMod ("→" with "ref") as (?) "(↦ &_& cl)". iModIntro. wp_store.
-    iModIntro. iApply fupdw_expand; [iApply tinv_wsat_incl|].
-    by iMod ("cl" with "↦ T") as "_".
+    iModIntro. by iMod ("cl" with "↦ T") as "_".
   Qed.
 
   (** Exchange on [ref[ ]] *)
@@ -84,11 +79,9 @@ Section eref.
     iIntros (?) "/= >(%&->& ref)". rewrite Loc.add_0.
     iApply (twpw_atomic (e:=Xchg _ _)); [done|]. iApply fupdw_tinv_wsat_le.
     iIntros (?). have ? : i <ⁿ L by exact (nlt_nle_trans _ _).
-    have ? : S i ≤ⁿ j by done. iApply fupdw_expand; [iApply tinv_wsat_incl|].
-    iDestruct tderiv_sound as "→".
+    iDestruct tderiv_sound as "→". have ? : S i ≤ⁿ j by done.
     iMod ("→" with "ref") as (?) "(↦ & ? & cl)". iModIntro. wp_xchg.
-    iModIntro. iApply fupdw_expand; [iApply tinv_wsat_incl|].
-    iMod ("cl" with "↦ T") as "_". by iFrame.
+    iModIntro. iMod ("cl" with "↦ T") as "_". by iFrame.
   Qed.
 
   (** Compare-exchange on [ref[ ]] *)
@@ -102,16 +95,14 @@ Section eref.
     iIntros (?) "/= >(%&->& ref)". rewrite Loc.add_0.
     iApply (twpw_atomic (e:=CmpXchg _ _ _)); [done|]. iApply fupdw_tinv_wsat_le.
     iIntros (?). have ? : i <ⁿ L by exact (nlt_nle_trans _ _).
-    have ? : S i ≤ⁿ j by done. iApply fupdw_expand; [iApply tinv_wsat_incl|].
-    iDestruct tderiv_sound as "→".
+    iDestruct tderiv_sound as "→". have ? : S i ≤ⁿ j by done.
     iMod ("→" with "ref") as (?) "(↦ &[%m' ->]& cl)". iModIntro.
     case (decide (m' = m)%Z)=> [->|?];
       [wp_apply (twp_cmpxchg_suc with "↦"); [done|solve_vals_compare_safe|]|
         wp_apply (twp_cmpxchg_fail with "↦");
           [case; lia|solve_vals_compare_safe|]];
-      iIntros "↦"; iApply fupdw_expand; try (by iApply tinv_wsat_incl);
-      iMod ("cl" with "↦ []") as "_"; try (by iExists _); iPureIntro;
-      eexists _, _; split=>//; split; by eexists.
+      iIntros "↦";  iMod ("cl" with "↦ []") as "_"; try (by iExists _);
+      iPureIntro; eexists _, _; split=>//; split; by eexists.
   Qed.
 
   (** Fetch-and-add on [ref[ ]] *)
@@ -123,11 +114,9 @@ Section eref.
     iIntros (?) "/= >(%&->& ref)". rewrite Loc.add_0.
     iApply (twpw_atomic (e:=FAA _ _)); [done|]. iApply fupdw_tinv_wsat_le.
     iIntros (?). have ? : i <ⁿ L by exact (nlt_nle_trans _ _).
-    have ? : S i ≤ⁿ j by done. iApply fupdw_expand; [iApply tinv_wsat_incl|].
-    iDestruct tderiv_sound as "→".
+    iDestruct tderiv_sound as "→". have ? : S i ≤ⁿ j by done.
     iMod ("→" with "ref") as (?) "(↦ &(%m &->)& cl)". iModIntro. wp_faa.
-    iModIntro. iApply fupdw_expand; [iApply tinv_wsat_incl|].
-    rewrite -Nat2Z.inj_add.
+    iModIntro. rewrite -Nat2Z.inj_add.
     iMod ("cl" with "↦ []") as "_"; [|do 2 iModIntro]; by iExists _.
   Qed.
 End eref.
